examples/proofs/intptr/generated_proof_roundtrip_and_read2.v
@@ -1,0 +1,25 @@
+From refinedc.typing Require Import typing.
+From refinedc.examples.intptr Require Import generated_code.
+From refinedc.examples.intptr Require Import generated_spec.
+Set Default Proof Using "Type".
+
+(* Generated from [examples/intptr.c]. *)
+Section proof_roundtrip_and_read2.
+  Context `{!typeG Σ} `{!globalG Σ}.
+
+  (* Typing proof for [roundtrip_and_read2]. *)
+  Lemma type_roundtrip_and_read2 :
+    ⊢ typed_function impl_roundtrip_and_read2 type_of_roundtrip_and_read2.
+  Proof.
+    start_function "roundtrip_and_read2" ([p n]) => arg_p local_i local_q.
+    split_blocks ((
+      ∅
+    )%I : gmap label (iProp Σ)) ((
+      ∅
+    )%I : gmap label (iProp Σ)).
+    - repeat liRStep; liShow.
+      all: print_typesystem_goal "roundtrip_and_read2" "#0".
+    Unshelve. all: sidecond_hook; prepare_sideconditions; normalize_and_simpl_goal; try solve_goal; unsolved_sidecond_hook.
+    all: print_sidecondition_goal "roundtrip_and_read2".
+  Qed.
+End proof_roundtrip_and_read2.
